Congruence_Closure_Explain/CC_Explain.thy
@@ -5,16 +5,16 @@ begin
 
 subsection \<open>Explain definition\<close>
 
-text \<open>The highest node is in this case the same as the rep_of, because we do not 
+text \<open>The "highest node" is in this case the same as the rep_of, because we do not 
       have the optimisation of checking which equivalence class is bigger, 
       we just make the union in the given order. When adding this optimisation,
       a highest_node function must be also implemented. \<close>
 
 text \<open>There are three variables changed by the function \<open>explain_along_path\<close>: 
 
-      The overall output of explain
-      The Union Find list of the additional union find, which is local to the explain function
-      The list of pending proofs, which need to be recursively called with cc_explain
+    * The overall output of explain
+    * The Union Find list of the additional union find, which is local to the explain function
+    * The list of pending proofs, which need to be recursively called with cc_explain
       
       These are the three values returned by this function.\<close>
 
@@ -55,28 +55,22 @@ lemma explain_along_path_simp2:
     "(pf_labels cc) ! rep_of l a = Some (One a')"
     "(output, new_l, pend) = explain_along_path cc (ufa_union l a ((proof_forest cc) ! rep_of l a)) 
      ((proof_forest cc) ! rep_of l a) c"
+    "explain_along_path_dom (cc, l, a, c)"
   shows "explain_along_path cc l a c = ({a'} \<union> output, new_l, pend)"
-proof-
-  have "explain_along_path_dom (cc, l, a, c)"
-    using assms explain_along_path.domintros sorry
-  then show ?thesis using explain_along_path.psimps unfolding Let_def
+ using explain_along_path.psimps unfolding Let_def
     by (metis (no_types, lifting) assms case_prod_conv option.sel pending_equation.simps(5))
-qed
+
 
 lemma explain_along_path_simp3:
   assumes "rep_of l a \<noteq> rep_of l c"
     "(pf_labels cc) ! rep_of l a = Some (Two (F a\<^sub>1 a\<^sub>2 \<approx> a') (F b\<^sub>1 b\<^sub>2 \<approx> b'))"
     "explain_along_path cc (ufa_union l a ((proof_forest cc) ! rep_of l a)) 
      ((proof_forest cc) ! rep_of l a) c = (output, new_l, pend)"
+    "explain_along_path_dom (cc, l, a, c)"
   shows "explain_along_path cc l a c = ({(F a\<^sub>1 a\<^sub>2 \<approx> a'), (F b\<^sub>1 b\<^sub>2 \<approx> b')} \<union> output, 
          new_l, [(a\<^sub>1, b\<^sub>1), (a\<^sub>2, b\<^sub>2)] @ pend)"
-proof-
-  have "explain_along_path_dom (cc, l, a, c)"
-    using assms explain_along_path.domintros sorry
-  then show ?thesis using explain_along_path.psimps unfolding Let_def
-    using assms case_prod_conv option.sel pending_equation.simps(6) equation.simps(6) 
-    by (metis (no_types, lifting))
-qed
+  using explain_along_path.psimps unfolding Let_def
+    by (metis (no_types, lifting) assms case_prod_conv option.sel pending_equation.simps(6) equation.simps(6))
 
 function cc_explain_aux :: "congruence_closure \<Rightarrow> nat list \<Rightarrow> (nat * nat) list \<Rightarrow> equation set"
   where
@@ -85,8 +79,8 @@ function cc_explain_aux :: "congruence_closure \<Rightarrow> nat list \<Rightarr
 (if are_congruent cc (a \<approx> b)
 then
   (let c = lowest_common_ancestor (proof_forest cc) a b;
-   (output1, new_l, pending1) = explain_along_path cc l a c;
-   (output2, new_new_l, pending2) = explain_along_path cc new_l b c
+    (output1, new_l, pending1) = explain_along_path cc l a c;
+    (output2, new_new_l, pending2) = explain_along_path cc new_l b c
   in
     output1 \<union> output2 \<union> cc_explain_aux cc new_new_l (xs @ pending1 @ pending2))
 else cc_explain_aux cc l xs)
@@ -97,265 +91,187 @@ fun cc_explain :: "congruence_closure \<Rightarrow> nat \<Rightarrow> nat \<Righ
   where
 "cc_explain cc a b = cc_explain_aux cc [0..<nr_vars cc] [(a, b)]"
 
-subsection \<open>Invariant for the additional union find in cc_explain\<close>
-
-definition explain_list_invar :: "nat list \<Rightarrow> nat list \<Rightarrow> bool"
-  where
-\<comment> \<open>They have the same rep\<close>
-"explain_list_invar l pf \<equiv> (\<forall> i < length l. l ! i \<noteq> i \<longrightarrow> l ! i = pf ! i) \<and> 
-(length l = length pf)"
-
-lemma explain_list_invar_paths: 
-"path l a p b \<Longrightarrow> explain_list_invar l pf \<Longrightarrow> path pf a p b"
-proof(induction rule: path.induct)
-  case (single n l)
-  then show ?case 
-    by (simp add: explain_list_invar_def path.single)
-next
-  case (step r l u p v)
-  then show ?case unfolding explain_list_invar_def 
-    by (metis path.step path_nodes_lt_length_l)
-qed
-
-lemma explain_list_invar_initial:
-"explain_list_invar [0..<n] [0..<n]"
-  unfolding explain_list_invar_def by blast
-
-lemma explain_list_invar_union:
-  assumes "explain_list_invar l pf" "a < length l"
-  shows "explain_list_invar (ufa_union l a (pf ! rep_of l a)) pf"
-  unfolding explain_list_invar_def 
-proof(standard, standard, standard, standard)
-  fix i
-  assume prems: "i < length (ufa_union l a (pf ! rep_of l a))"
-"ufa_union l a (pf ! rep_of l a) ! i \<noteq> i"
-  show "ufa_union l a (pf ! rep_of l a) ! i = pf ! i"
-  proof(cases "i = rep_of l a")
-    case True
-    have "rep_of l a < length l" 
-      using True prems(1) by auto
-    with True have "ufa_union l a (pf ! rep_of l a) ! i = rep_of l (pf ! rep_of l a)" 
-      by simp
-    then show ?thesis sorry
-  next
-    case False
-    then show ?thesis using assms(1) prems unfolding explain_list_invar_def by simp
-  qed
-next 
-  show "length (ufa_union l a (pf ! rep_of l a)) = length pf" 
-    using assms(1) unfolding explain_list_invar_def by simp
-qed
-
-lemma explain_list_invar_explain_along_path:
-"True"
-  sorry
-
-text "To show about pfl: left a = i and right a = pf ! i or opposite
-also it's never None if pf ! i ~= i."
+text \<open>TODO: To show about pfl: left a = i and right a = pf ! i or opposite
+also it's never None if pf ! i ~= i.\<close>
 
 subsection \<open>Correctness of \<open>explain_along_path\<close>\<close>
+
+text \<open>This function is needed in order to interpret the pending list of the explain
+operation as a set of equations.\<close>
 fun pending_set_explain :: "(nat * nat) list \<Rightarrow> equation set"
   where
     "pending_set_explain pend = set (map (\<lambda>(a, b) . (a \<approx> b)) pend)"
 
 lemma pending_set_explain_Cons:
-  "pending_set_explain ((a,b) # pend) = {(a \<approx> b)} \<union> pending_set_explain pend"
+  "pending_set_explain ((a, b) # pend) = {(a \<approx> b)} \<union> pending_set_explain pend"
   by auto
 
 lemma explain_along_path_correctness:
-  assumes "ufa_invar pf"
+  assumes "explain_along_path_dom (\<lparr>cc_list = cc_l, use_list = u, lookup = t, pending = pe, 
+proof_forest = pf, pf_labels = pfl, input = ip\<rparr>, l, a, c)"
+(is "explain_along_path_dom (?cc, l, a, c)")
+    "ufa_invar pf"
     "a < length pf"
     "c < length pf"
     "ufa_invar l"
-    "path pf c pAC a"
     "length l = length pf"
     "explain_along_path \<lparr>cc_list = cc_l, use_list = u, lookup = t, pending = pe, 
 proof_forest = pf, pf_labels = pfl, input = ip\<rparr> l a c = (output, new_l, pend)"
+"path pf c pAC a"
+"pf_labels_invar \<lparr>cc_list = cc_l, use_list = u, lookup = t, pending = pe, 
+proof_forest = pf, pf_labels = pfl, input = ip\<rparr>"
   shows "(a \<approx> c) \<in> Congruence_Closure (representatives_set l \<union> output 
 \<union> pending_set_explain pend)"
-  using assms proof(induction "length pAC" arbitrary: "output" new_l pend l pAC a rule: less_induct)
-  case less
-  then show ?case proof(cases "pf ! a = a")
+  using assms proof(induction "\<lparr>cc_list = cc_l, use_list = u, lookup = t, pending = pe, 
+proof_forest = pf, pf_labels = pfl, input = ip\<rparr>"
+    l a c arbitrary: pAC "output" new_l pend rule: explain_along_path.pinduct)
+  case (1 l a c)
+  then show ?case proof(cases "rep_of l a = rep_of l c")
     case True
-    with less have "c = a" using path_root by auto
-    then show ?thesis by blast
+    then have "(a \<approx> c) \<in> Congruence_Closure (representatives_set l)"
+      using CC_same_rep_representatives_set[of l a c] 1 by argo
+    then show ?thesis 
+      using Congruence_Closure_split_rule by auto
   next
     case False
-    then show ?thesis proof(cases "rep_of l a = rep_of l c")
-      case True
-      then have "(a \<approx> c) \<in> Congruence_Closure (representatives_set l)"
-        using CC_same_rep_representatives_set[of l a c] less by argo
-      then show ?thesis 
-        using Congruence_Closure_split_rule by auto
-    next
-      case False': False
-      then obtain paRoot where paRoot: "path l (rep_of l a) paRoot a" 
-        using less False by (metis path_to_root_correct) 
-      then have *: "path pf (rep_of l a) paRoot a" sorry (*1*)
-      have length_pAC: "length paRoot < length pAC" 
-      proof(rule ccontr)
-        \<comment> \<open>If paRoot was longer than pAC, then there would be a path
-from a to c in the additional union find (l), 
-therefore a and c would have the same representative, which is a contradiction.\<close>
-        let ?pARfront = "take (length paRoot - length pAC + 1) paRoot"
-        let ?pARback = "drop (length paRoot - length pAC + 1) paRoot"
-        assume length_p: "\<not> length paRoot < length pAC"
-        then have not_empty: "?pARfront \<noteq> []" 
-          by (metis "*" add_nonneg_eq_0_iff less_eq_nat.simps(1) path_properties take_eq_Nil2 zero_neq_one)
-        with paRoot have p: "path l (rep_of l a) (?pARfront @ ?pARback) a"
-          by auto
-        then have path_pf_to_a: "path l (rep_of l a) (?pARfront) (last ?pARfront)"
-          "path l (last ?pARfront) (last ?pARfront # ?pARback) a"
-          using path_divide1[OF p not_empty] by blast+
-        then have path_pf_to_a: "path pf (last ?pARfront) (last ?pARfront # ?pARback) a"
-          sorry (*1*)
-        then have "length (last ?pARfront # ?pARback) = length pAC" 
-          by (metis (no_types, lifting) One_nat_def Suc_diff_1 ab_semigroup_add_class.add.commute add_diff_cancel_right add_diff_inverse_nat drop0 drop_Suc_Cons length_drop length_greater_0_conv length_p less.prems(5) list.discI path.simps)
-        then have "c = last ?pARfront" 
-          using less.prems(1,5) path_pf_to_a path_unique_if_length_eq by blast
-        then have "rep_of l c = rep_of l a" 
-          using less.prems(4) not_empty p path_divide1 path_rep_eq by blast
-        then show "False"
-          using False' by auto
-      qed
-      let ?pRootC = "(take (length pAC - length paRoot + 1) pAC)"
-      from length_pAC have "path pf c ?pRootC (rep_of l a)" 
-        using * less path_longer by fast
-      with less path_butlast have path_to_parent: "path pf c (butlast ?pRootC) (pf ! rep_of l a)" 
-        by (metis False' \<open>path l (rep_of l a) paRoot a\<close> path_rep_eq)
-      have "length paRoot > 0"
-        by (metis "*" length_greater_0_conv path_not_empty)
-      then have "length pAC - length paRoot + 1 \<le> length pAC"  
-        using length_pAC by linarith
-      then have length_pRootC: "length (butlast ?pRootC) < length pAC"  
-        by simp
-      obtain output' new_l' pend' where recursive_step: "
-explain_along_path
-     \<lparr>cc_list = cc_l, use_list = u, lookup = t, pending = pe, proof_forest = pf, 
-pf_labels = pfl, input = ip\<rparr>
+    obtain output' new_l' pend' where recursive_step: "explain_along_path ?cc
      (ufa_union l a (pf ! rep_of l a)) (pf ! rep_of l a) c = (output', new_l', pend')"
-        using prod_cases3 by blast
-      have valid: "(pf ! rep_of l a) < length pf" "ufa_invar (ufa_union l a (pf ! rep_of l a))"
-        using "*" less.prems(1,4,6) path_nodes_lt_length_l ufa_invarD(2) ufa_union_invar by auto
-      with less(1)[OF length_pRootC less(2) this(1) less(4) this(2) path_to_parent] 
-        path_to_parent recursive_step have IH: "(pf ! rep_of l a \<approx> c) \<in>
- Congruence_Closure (representatives_set (ufa_union l a (pf ! rep_of l a)) \<union> output'
-\<union> pending_set_explain pend')" using less(7) by auto
-      then have 3: "((pf ! rep_of l a) \<approx> (rep_of l a)) \<in> Congruence_Closure
-        (representatives_set l \<union> output \<union> pending_set_explain pend) \<Longrightarrow>
-output' \<subseteq> output \<Longrightarrow> pending_set_explain pend' \<subseteq> pending_set_explain pend \<Longrightarrow> 
-((pf ! rep_of l a) \<approx> c) \<in> Congruence_Closure
-        (representatives_set l \<union> output \<union> pending_set_explain pend)"
-      proof(rule Congruence_Closure_imp)
-        fix eq
-        let ?union = "(ufa_union l a (pf ! rep_of l a))"
-        assume prems: "eq \<in> representatives_set ?union \<union> output' \<union> pending_set_explain pend'"
-          "((pf ! rep_of l a) \<approx> (rep_of l a))
-         \<in> Congruence_Closure (representatives_set l \<union> output \<union> pending_set_explain pend)"
-          "output' \<subseteq> output" "pending_set_explain pend' \<subseteq> pending_set_explain pend"
-        then consider (output_or_pending) "eq \<in> output' \<union> pending_set_explain pend'"
-          | (rep_set) k where "eq = (k \<approx> rep_of ?union k)" "k < length ?union" "?union ! k \<noteq> k"
-          by blast
-        then show "eq \<in> Congruence_Closure (representatives_set l \<union> output \<union> pending_set_explain pend)"
-        proof(cases)
-          case output_or_pending
-          then show ?thesis
-            using prems by blast
-        next
-          case rep_set
-          then obtain pathRK where pathRK: "path ?union (rep_of ?union k) pathRK k"
-            using valid(2) path_to_root_correct by blast
-          then show ?thesis proof(cases "rep_of l a = rep_of l k")
-            case True
-              \<comment> \<open>If they are in rep_set: in l: \<open>rep_of l a\<close> has the same rep as \<open>a\<close>,
-and \<open>pf ! rep_of l a\<close> has the same rep as \<open>rep_of ?union k\<close>, and 
-\<open>rep_of l a\<close> and \<open>a\<close> are congruent as an assumption.\<close>
-            then have "rep_of l (pf ! rep_of l a) = rep_of ?union k"
-              using less.prems(4,6) rep_set(2) ufa_union_aux valid(1) by auto
-            then have
-              *: "((pf ! rep_of l a) \<approx> (rep_of ?union k))
-\<in> Congruence_Closure (representatives_set l \<union> output \<union> pending_set_explain pend)"
-              by (metis (no_types, lifting) Congruence_Closure.symmetric Congruence_Closure_split_rule a_eq_rep_of_a_in_CC_representatives_set(2) less.prems(6) valid(1))
-            then have
-              "(k \<approx> rep_of l a)
-\<in> Congruence_Closure (representatives_set l \<union> output \<union> pending_set_explain pend)"
-              by (metis (no_types, lifting) symmetric Congruence_Closure_split_rule True a_eq_rep_of_a_in_CC_representatives_set(2) length_list_update rep_set(2))
-            with * show ?thesis 
-              using prems by (metis (no_types, lifting) symmetric transitive1 rep_set(1))
-          next
-            case False
-            then have "rep_of ?union k = rep_of l k" 
-              by (metis length_list_update less.prems(4,6) paRoot path_nodes_lt_length_l rep_set(2) ufa_union_aux valid(1))
-            then show ?thesis 
-              using symmetric Congruence_Closure_split_rule a_eq_rep_of_a_in_CC_representatives_set(2) rep_set by force
-          qed 
-        qed 
-      qed
-      have "(a \<approx> (rep_of l a)) \<in> Congruence_Closure (representatives_set l)"
-        by (auto simp add: less.prems(2) less.prems(4) less.prems(6) rep_of_iff)
-      then have 1: "(a \<approx> rep_of l a) \<in> Congruence_Closure 
+      using prod_cases3 by blast
+    have valid: "(pf ! rep_of l a) < length pf" "ufa_invar (ufa_union l a (pf ! rep_of l a))"
+      using "1.prems" path_nodes_lt_length_l ufa_invarD(2) ufa_union_invar by (metis rep_of_bound)+
+    have "(a \<approx> (rep_of l a)) \<in> Congruence_Closure (representatives_set l)"
+      by (auto simp add: "1.prems" rep_of_iff)
+    then have 4: "(a \<approx> (rep_of l a)) \<in> Congruence_Closure 
 (representatives_set l \<union> output \<union> pending_set_explain pend)"
-        using Congruence_Closure_split_rule by auto
-      show ?thesis proof(cases "the (pfl ! rep_of l a)")
-        case (One a')
-        then have *: "pfl ! rep_of l a = Some (One a')" sorry (*3*)
-            (*TODO add pfl invar, similar to pending invar*)
-        have dom: "explain_along_path_dom
-     (\<lparr>cc_list = cc_l, use_list = u, lookup = t, pending = pe, 
-proof_forest = pf, pf_labels = pfl, input = ip\<rparr>, 
-l,a, c)" sorry 
-        have result: "(output, new_l, pend) = ({a'} \<union> output', new_l', pend')" 
-          using less(8) explain_along_path_simp2[OF False'] One 
-            False * recursive_step by auto
-        then have a': "a' = (rep_of l a \<approx> pf ! rep_of l a)
-\<or> a' = (pf ! rep_of l a \<approx> rep_of l a)" sorry (*3*)
-        have "(rep_of l a \<approx> pf ! rep_of l a) \<in> 
-Congruence_Closure ({a'} \<union> output')" 
-          using a' by blast
-        then have 2: "(rep_of l a \<approx> pf ! rep_of l a) \<in> 
-Congruence_Closure (representatives_set l \<union> output \<union> pending_set_explain pend)"
-          using result Congruence_Closure_split_rule 
-          by (metis (no_types, lifting) Pair_inject sup_commute)
-        from result have "representatives_set l \<union> output' \<union> pending_set_explain pend'
-\<subseteq> representatives_set l \<union> output \<union> pending_set_explain pend" 
-          by blast
-        with 3 have "(pf ! rep_of l a \<approx> c) \<in> Congruence_Closure
+      using Congruence_Closure_split_rule by auto
+    \<comment> \<open>If \<open>(pf ! rep_of l a) \<approx> c\<close> is in the congruence closure of the recursive call, 
+        then it will also be in the congruence closure of the output.\<close>
+    let ?union = "(ufa_union l a (pf ! rep_of l a))"
+    have cc_output: "((pf ! rep_of l a) \<approx> c) \<in>
+ Congruence_Closure (representatives_set ?union \<union> output'
+\<union> pending_set_explain pend')
+\<Longrightarrow> ((pf ! rep_of l a) \<approx> (rep_of l a)) \<in> Congruence_Closure
+        (representatives_set l \<union> output \<union> pending_set_explain pend) 
+\<Longrightarrow> output' \<subseteq> output
+\<Longrightarrow> pending_set_explain pend' \<subseteq> pending_set_explain pend 
+\<Longrightarrow> ((pf ! rep_of l a) \<approx> c) \<in> Congruence_Closure
         (representatives_set l \<union> output \<union> pending_set_explain pend)"
-          using Congruence_Closure_monotonic 2 symmetric result by blast
-        then show ?thesis using 1 2 by blast
+    proof(rule Congruence_Closure_imp)
+      fix eq
+      assume prems: "eq \<in> representatives_set ?union \<union> output' \<union> pending_set_explain pend'"
+        "((pf ! rep_of l a) \<approx> (rep_of l a))
+         \<in> Congruence_Closure (representatives_set l \<union> output \<union> pending_set_explain pend)"
+        "output' \<subseteq> output" "pending_set_explain pend' \<subseteq> pending_set_explain pend"
+      then consider (output_or_pending) "eq \<in> output' \<union> pending_set_explain pend'"
+        | (rep_set) k where "eq = (k \<approx> rep_of ?union k)" "k < length ?union" "?union ! k \<noteq> k"
+        by blast                      
+      then show "eq \<in> Congruence_Closure (representatives_set l \<union> output \<union> pending_set_explain pend)"
+      proof(cases)
+        case output_or_pending
+        then show ?thesis
+          using prems by blast
       next
-        case (Two x21 x22)
-        then obtain a\<^sub>1 a\<^sub>2 a' b\<^sub>1 b\<^sub>2 b' where *: "(pfl ! rep_of l a)
-= Some (Two (F a\<^sub>1 a\<^sub>2 \<approx> a') (F b\<^sub>1 b\<^sub>2 \<approx> b'))" sorry (*3*)
-        have dom: "explain_along_path_dom
-     (\<lparr>cc_list = cc_l, use_list = u, lookup = t, pending = pe, 
-proof_forest = pf, pf_labels = pfl, input = ip\<rparr>, 
-l, a, c)" sorry (*4*)
-        have result: "(output, new_l, pend) = 
+        case rep_set
+        then obtain pathRK where pathRK: "path ?union (rep_of ?union k) pathRK k"
+          using valid(2) path_to_root_correct by blast
+        then show ?thesis proof(cases "rep_of l a = rep_of l k")
+          case True
+            \<comment> \<open>If they are in rep_set: in l: \<open>rep_of l a\<close> has the same rep as \<open>a\<close>,
+                and \<open>pf ! rep_of l a\<close> has the same rep as \<open>rep_of ?union k\<close>, and 
+                \<open>rep_of l a\<close> and \<open>a\<close> are congruent by assumption.\<close>
+          then have "rep_of l (pf ! rep_of l a) = rep_of ?union k"
+            using "1.prems" rep_set(2) ufa_union_aux valid(1) by auto
+          with "1.prems" have
+            *: "((pf ! rep_of l a) \<approx> (rep_of ?union k))
+\<in> Congruence_Closure (representatives_set l \<union> output \<union> pending_set_explain pend)"
+            by (metis (no_types, lifting) Congruence_Closure.symmetric Congruence_Closure_split_rule a_eq_rep_of_a_in_CC_representatives_set(2) valid(1))
+          then have
+            "(k \<approx> (rep_of l a))
+\<in> Congruence_Closure (representatives_set l \<union> output \<union> pending_set_explain pend)"
+            by (metis (no_types, lifting) symmetric Congruence_Closure_split_rule True a_eq_rep_of_a_in_CC_representatives_set(2) length_list_update rep_set(2))
+          with * show ?thesis 
+            using prems by (metis (no_types, lifting) symmetric transitive1 rep_set(1))
+        next
+          case False
+          with "1.prems" have "rep_of ?union k = rep_of l k" 
+            by (metis length_list_update rep_set(2) ufa_union_aux valid(1))
+          then show ?thesis 
+            using symmetric Congruence_Closure_split_rule a_eq_rep_of_a_in_CC_representatives_set(2) rep_set by force
+        qed 
+      qed 
+    qed
+    obtain pRAC where pRAC: "path pf c pRAC (rep_of l a)"sorry
+    then have pRAC': "path pf c (butlast pRAC) (pf ! rep_of l a)"
+        by (metis "1.prems"(2) "1.prems"(4) "1.prems"(5) False path_butlast rep_of_idem)
+      from pRAC have "pf ! rep_of l a \<noteq> rep_of l a" using "1.prems"(7)
+        by (metis "1.prems"(2) "1.prems"(4) "1.prems"(5) False path_root rep_of_min rep_of_refl)
+      then obtain aa a\<^sub>1 a\<^sub>2 bb b\<^sub>1 b\<^sub>2 where valid_eq: "
+(pfl ! rep_of l a = Some (One (aa \<approx> bb)) \<or> 
+          pfl ! rep_of l a = Some (Two (F a\<^sub>1 a\<^sub>2 \<approx> aa) (F b\<^sub>1 b\<^sub>2 \<approx> bb)))
+          \<and> (aa = pf ! rep_of l a \<and> bb = rep_of l a \<or> aa = rep_of l a \<and> bb = pf ! rep_of l a)
+        "using "1.prems" unfolding pf_labels_invar_def congruence_closure.select_convs(*3*) 
+        by (metis rep_of_less_length_l)
+    show ?thesis proof(cases "the (pfl ! rep_of l a)")
+      case (One a')
+      from valid_eq have *: "pfl ! rep_of l a = Some (One a')" 
+        using One by auto
+      with recursive_step 1(2)[OF False] have IH: 
+        "(pf ! rep_of l a \<approx> c) \<in>
+ Congruence_Closure (representatives_set (ufa_union l a (pf ! rep_of l a)) \<union> output'
+\<union> pending_set_explain pend')" 
+        using "1.prems" One valid pRAC' by simp
+      have result: "(output, new_l, pend) = ({a'} \<union> output', new_l', pend')" 
+        using 1 explain_along_path_simp2[OF False] One False * recursive_step by auto
+      then have a': "a' = (rep_of l a \<approx> pf ! rep_of l a)
+\<or> a' = (pf ! rep_of l a \<approx> rep_of l a)" 
+        using One valid_eq by auto
+      then have "(rep_of l a \<approx> pf ! rep_of l a) \<in> 
+Congruence_Closure ({a'} \<union> output')" 
+        by blast
+      with result have 2: "(rep_of l a \<approx> pf ! rep_of l a) \<in> 
+Congruence_Closure (representatives_set l \<union> output \<union> pending_set_explain pend)"
+        using Congruence_Closure_split_rule by (metis (no_types, lifting) Pair_inject sup_commute)
+      from result have "output' \<subseteq> output"  "pending_set_explain pend' \<subseteq> pending_set_explain pend "
+        by blast+
+      with cc_output have 3: "(pf ! rep_of l a \<approx> c) \<in> Congruence_Closure
+        (representatives_set l \<union> output \<union> pending_set_explain pend)" 
+        using "2" IH by blast
+      from 2 3 4 show ?thesis by blast
+    next
+      case (Two x21 x22)
+      then obtain a\<^sub>1 a\<^sub>2 a' b\<^sub>1 b\<^sub>2 b' where *: "(pfl ! rep_of l a)
+= Some (Two (F a\<^sub>1 a\<^sub>2 \<approx> a') (F b\<^sub>1 b\<^sub>2 \<approx> b'))" 
+        by (metis option.sel pending_equation.distinct(1) valid_eq) 
+      with recursive_step 1(3)[OF False] have IH: 
+        "(pf ! rep_of l a \<approx> c) \<in>
+ Congruence_Closure (representatives_set (ufa_union l a (pf ! rep_of l a)) \<union> output'
+\<union> pending_set_explain pend')" 
+        using * pRAC' by (simp add: "1.prems" Two valid)
+      have result: "(output, new_l, pend) = 
 ({(F a\<^sub>1 a\<^sub>2 \<approx> a'), (F b\<^sub>1 b\<^sub>2 \<approx> b')} \<union> output', new_l', [(a\<^sub>1, b\<^sub>1), (a\<^sub>2, b\<^sub>2)] @ pend')" 
-          using less(8) explain_along_path_simp3[OF False']
-            False * recursive_step by auto
-        then have a': "a' = rep_of l a \<and> b' = pf ! rep_of l a
-\<or> a' = pf ! rep_of l a \<and> b' = rep_of l a" sorry (*3*)
-        have "(a\<^sub>1 \<approx> b\<^sub>1) \<in> Congruence_Closure (representatives_set l \<union> output \<union> pending_set_explain pend)"
-          "(a\<^sub>2 \<approx> b\<^sub>2) \<in> Congruence_Closure (representatives_set l \<union> output \<union> pending_set_explain pend)"
-          "(F a\<^sub>1 a\<^sub>2 \<approx> a') \<in> Congruence_Closure (representatives_set l \<union> output \<union> pending_set_explain pend)"
-          "(F b\<^sub>1 b\<^sub>2 \<approx> b') \<in> Congruence_Closure (representatives_set l \<union> output \<union> pending_set_explain pend)"
-          using result by auto
-        then have 2: "(rep_of l a \<approx> pf ! rep_of l a) \<in> 
+        using 1 explain_along_path_simp3[OF False] * recursive_step by auto
+      then have a': "a' = rep_of l a \<and> b' = pf ! rep_of l a
+\<or> a' = pf ! rep_of l a \<and> b' = rep_of l a" 
+        using valid_eq * by auto
+      have "(a\<^sub>1 \<approx> b\<^sub>1) \<in> Congruence_Closure (representatives_set l \<union> output \<union> pending_set_explain pend)"
+        "(a\<^sub>2 \<approx> b\<^sub>2) \<in> Congruence_Closure (representatives_set l \<union> output \<union> pending_set_explain pend)"
+        "(F a\<^sub>1 a\<^sub>2 \<approx> a') \<in> Congruence_Closure (representatives_set l \<union> output \<union> pending_set_explain pend)"
+        "(F b\<^sub>1 b\<^sub>2 \<approx> b') \<in> Congruence_Closure (representatives_set l \<union> output \<union> pending_set_explain pend)"
+        using result by auto
+      then have 2: "((rep_of l a) \<approx> (pf ! rep_of l a)) \<in> 
 Congruence_Closure (representatives_set l \<union> output \<union> pending_set_explain pend)" 
-          using a' monotonic by blast
-        from result have "representatives_set l \<union> output' \<union> pending_set_explain pend'
+        using a' monotonic by blast
+      from result have "representatives_set l \<union> output' \<union> pending_set_explain pend'
 \<subseteq> representatives_set l \<union> output \<union> pending_set_explain pend" 
-          using pending_set_explain_Cons by auto
-        with 3 have "(pf ! rep_of l a \<approx> c) \<in> Congruence_Closure
+        using pending_set_explain_Cons by auto
+      with cc_output have "((pf ! rep_of l a) \<approx> c) \<in> Congruence_Closure
         (representatives_set l \<union> output \<union> pending_set_explain pend)"
-          using Congruence_Closure_monotonic 2 symmetric result by auto
-        then show ?thesis using 1 2 by blast
-      qed
+        using Congruence_Closure_monotonic 2 result IH by auto 
+      then show ?thesis using 4 2 by blast
     qed
   qed
 qed
+
 
 subsection \<open>Correctness of explain\<close>
 
